multicore: strengthen top-m bridge and global EDF layer

theories/Abstractions/SchedulingAlgorithm/TopMSchedulerBridge.v
@@ -39,6 +39,14 @@ Definition top_m_algorithm_schedule
         else
           None).
 
+Definition top_m_algorithm_scheduler_on
+    (J : JobId -> Prop)
+    (spec : GenericTopMSchedulingAlgorithm)
+    (candidates_of : CandidateSource)
+    (_ : CandidateSourceSpec J candidates_of)
+    : Scheduler :=
+  top_m_algorithm_schedule spec candidates_of.
+
 (* ===== Helper lemma ===== *)
 
 Lemma nth_error_some_in :
@@ -48,6 +56,42 @@ Lemma nth_error_some_in :
 Proof.
   intros l n j H.
   exact (@nth_error_In JobId l n j H).
+Qed.
+
+Lemma in_nth_error_exists :
+  forall (l : list JobId) j,
+    In j l ->
+    exists n, nth_error l n = Some j.
+Proof.
+  intros l j Hin.
+  apply In_nth_error in Hin.
+  destruct Hin as [n Hnth].
+  exists n. exact Hnth.
+Qed.
+
+Lemma nth_error_some_lt_length :
+  forall (l : list JobId) n j,
+    nth_error l n = Some j ->
+    n < length l.
+Proof.
+  intros l n j Hnth.
+  apply nth_error_Some.
+  rewrite Hnth. discriminate.
+Qed.
+
+Lemma nth_error_none_of_idle_cpu :
+  forall spec candidates_of jobs m sched t c,
+    scheduler_rel (top_m_algorithm_schedule spec candidates_of) jobs m sched ->
+    c < m ->
+    sched t c = None ->
+    nth_error (choose_top_m spec jobs m sched t (candidates_of jobs m sched t)) c = None.
+Proof.
+  intros spec candidates_of jobs m sched t c Hrel Hlt Hidle.
+  pose proof (Hrel t c) as Heq.
+  apply Nat.ltb_lt in Hlt.
+  rewrite Hlt in Heq. simpl in Heq.
+  rewrite Hidle in Heq.
+  symmetry. exact Heq.
 Qed.
 
 (* ===== Scheduler relation unfolding ===== *)
@@ -139,4 +183,162 @@ Proof.
   pose proof (choose_top_m_nodup spec jobs m sched t (cands jobs m sched t)) as Hnodup.
   fold chosen in Hnodup.
   exact (nth_error_nodup_inj chosen c1 c2 j Hnodup Heq1 Heq2).
+Qed.
+
+Lemma top_m_algorithm_in_subset :
+  forall J spec candidates_of jobs m sched t c j,
+    CandidateSourceSpec J candidates_of ->
+    scheduler_rel (top_m_algorithm_schedule spec candidates_of) jobs m sched ->
+    c < m ->
+    sched t c = Some j ->
+    J j.
+Proof.
+  intros J spec candidates_of jobs m sched t c j Hcand Hrel Hlt Hrun.
+  destruct Hcand as [Hsound _ _].
+  pose proof (top_m_algorithm_eq_cpu spec candidates_of jobs m sched t c Hrel) as Heq.
+  apply Nat.ltb_lt in Hlt.
+  rewrite Hlt in Heq. simpl in Heq.
+  rewrite Hrun in Heq.
+  symmetry in Heq.
+  apply (Hsound jobs m sched t j).
+  eapply choose_top_m_in_candidates.
+  exact (nth_error_some_in _ _ _ Heq).
+Qed.
+
+Lemma top_m_algorithm_all_cpus_idle_if_no_subset_eligible :
+  forall J spec candidates_of jobs m sched t,
+    CandidateSourceSpec J candidates_of ->
+    scheduler_rel (top_m_algorithm_schedule spec candidates_of) jobs m sched ->
+    (forall j, J j -> ~ eligible jobs m sched j t) ->
+    all_cpus_idle m sched t.
+Proof.
+  intros J spec candidates_of jobs m sched t Hcand Hrel Hnone.
+  unfold all_cpus_idle, cpu_idle.
+  intros c Hlt.
+  destruct (sched t c) as [j|] eqn:Hcpu.
+  - exfalso.
+    pose proof (top_m_algorithm_in_subset J spec candidates_of jobs m sched t c j
+                  Hcand Hrel Hlt Hcpu) as Hj.
+    pose proof (top_m_algorithm_valid spec candidates_of jobs m sched Hrel) as Hvalid.
+    pose proof (Hvalid j t c Hlt Hcpu) as Helig.
+    exact (Hnone j Hj Helig).
+  - reflexivity.
+Qed.
+
+Lemma top_m_algorithm_some_cpu_busy_if_subset_eligible :
+  forall J spec candidates_of jobs m sched t,
+    CandidateSourceSpec J candidates_of ->
+    scheduler_rel (top_m_algorithm_schedule spec candidates_of) jobs m sched ->
+    0 < m ->
+    (exists j, J j /\ eligible jobs m sched j t) ->
+    exists c, c < m /\ cpu_busy sched t c.
+Proof.
+  intros J spec candidates_of jobs m sched t Hcand Hrel Hm [j [HJ Helig]].
+  destruct Hcand as [_ Hcomplete _].
+  set (chosen := choose_top_m spec jobs m sched t (candidates_of jobs m sched t)).
+  assert (Hincand : In j (candidates_of jobs m sched t)).
+  { apply (Hcomplete jobs m sched t j HJ Helig). }
+  destruct (in_dec Nat.eq_dec j chosen) as [Hin|Hnotin].
+  - destruct (in_nth_error_exists chosen j Hin) as [c Hnth].
+    exists c. split.
+    + pose proof (nth_error_some_lt_length chosen c j Hnth) as Hclt.
+      pose proof (choose_top_m_length_le_m spec jobs m sched t (candidates_of jobs m sched t))
+        as Hlen.
+      unfold chosen in Hclt.
+      lia.
+    + exists j.
+      pose proof (top_m_algorithm_eq_cpu spec candidates_of jobs m sched t c Hrel) as Heq.
+      assert (Hlt : c < m).
+      { pose proof (nth_error_some_lt_length chosen c j Hnth) as Hclt.
+        pose proof (choose_top_m_length_le_m spec jobs m sched t (candidates_of jobs m sched t))
+          as Hlen.
+        unfold chosen in Hclt.
+        lia. }
+      apply Nat.ltb_lt in Hlt.
+      rewrite Hlt in Heq. simpl in Heq.
+      fold chosen in Heq.
+      rewrite Hnth in Heq.
+      exact Heq.
+  - assert (Hfull : length chosen = m).
+    { unfold chosen.
+      eapply choose_top_m_complete_if_room; eauto. }
+    destruct chosen as [|j0 chosen'] eqn:Hchosen.
+    + simpl in Hfull. lia.
+    + exists 0. split.
+      * exact Hm.
+      * exists j0.
+        pose proof (top_m_algorithm_eq_cpu spec candidates_of jobs m sched t 0 Hrel) as Heq.
+        apply Nat.ltb_lt in Hm.
+        rewrite Hm in Heq. simpl in Heq.
+        fold chosen in Heq.
+        rewrite Hchosen in Heq. simpl in Heq.
+        exact Heq.
+Qed.
+
+Lemma top_m_algorithm_running_if_some_cpu_idle_and_subset_eligible :
+  forall J spec candidates_of jobs m sched t j,
+    CandidateSourceSpec J candidates_of ->
+    scheduler_rel (top_m_algorithm_schedule spec candidates_of) jobs m sched ->
+    some_cpu_idle m sched t ->
+    J j ->
+    eligible jobs m sched j t ->
+    running m sched j t.
+Proof.
+  intros J spec candidates_of jobs m sched t j Hcand Hrel [c [Hclt Hidle]] HJ Helig.
+  destruct Hcand as [_ Hcomplete _].
+  set (chosen := choose_top_m spec jobs m sched t (candidates_of jobs m sched t)).
+  assert (Hincand : In j (candidates_of jobs m sched t)).
+  { apply (Hcomplete jobs m sched t j HJ Helig). }
+  assert (Hin : In j chosen).
+  { destruct (in_dec Nat.eq_dec j chosen) as [Hin|Hnotin].
+    - exact Hin.
+    - assert (Hfull : length chosen = m).
+      { unfold chosen.
+        eapply choose_top_m_complete_if_room; eauto. }
+      pose proof (nth_error_none_of_idle_cpu spec candidates_of jobs m sched t c Hrel Hclt Hidle)
+        as Hnthnone.
+      fold chosen in Hnthnone.
+      rewrite nth_error_None in Hnthnone.
+      rewrite Hfull in Hnthnone.
+      lia. }
+  destruct (in_nth_error_exists chosen j Hin) as [c' Hnth].
+  exists c'. split.
+  - pose proof (nth_error_some_lt_length chosen c' j Hnth) as Hlt.
+    pose proof (choose_top_m_length_le_m spec jobs m sched t (candidates_of jobs m sched t))
+      as Hlen.
+    unfold chosen in Hlt.
+    lia.
+  - pose proof (top_m_algorithm_eq_cpu spec candidates_of jobs m sched t c' Hrel) as Heq.
+    assert (Hlt : c' < m).
+      { pose proof (nth_error_some_lt_length chosen c' j Hnth) as Hlen'.
+        pose proof (choose_top_m_length_le_m spec jobs m sched t (candidates_of jobs m sched t))
+          as Hchosenlen.
+        unfold chosen in Hlen'.
+        lia. }
+    apply Nat.ltb_lt in Hlt.
+    rewrite Hlt in Heq. simpl in Heq.
+    fold chosen in Heq.
+    rewrite Hnth in Heq.
+    exact Heq.
+Qed.
+
+Lemma top_m_algorithm_schedulable_by_on_intro :
+  forall J spec candidates_of cand_spec jobs m sched,
+    scheduler_rel
+      (top_m_algorithm_scheduler_on J spec candidates_of cand_spec)
+      jobs m sched ->
+    feasible_schedule_on J jobs m sched ->
+    schedulable_by_on
+      J
+      (top_m_algorithm_scheduler_on J spec candidates_of cand_spec)
+      jobs m.
+Proof.
+  intros J spec candidates_of cand_spec jobs m sched Hrel Hfeas.
+  apply (schedulable_by_on_intro
+           J
+           (top_m_algorithm_scheduler_on J spec candidates_of cand_spec)
+           jobs m sched).
+  - exact Hrel.
+  - exact (top_m_algorithm_valid spec candidates_of jobs m sched Hrel).
+  - exact Hfeas.
 Qed.
